Refinement.thy
@@ -77,21 +77,99 @@ subsection \<open>RightPass\<close>
 definition removeEdge :: "_ graph \<Rightarrow> edge \<Rightarrow> _ graph" where
   "removeEdge c e \<equiv> c(e := 0)"
 
-(* TODO check definition *)
-definition rightPassRefine :: "_ graph \<Rightarrow> edge set \<Rightarrow> (_ graph) nres" where
-  "rightPassRefine c Q \<equiv> do {
+definition removeEdges :: "_graph \<Rightarrow> edge set \<Rightarrow> _ graph" where
+  "removeEdges c R \<equiv> \<lambda>e. if e \<in> R then 0 else c e"
+
+(* TODO refine removeEdges and use the refined version *)
+
+(* This is the exact definition, using the edge set*)
+definition rightPassRefine' :: "_ graph \<Rightarrow> edge set \<Rightarrow> (_ graph) nres" where
+  "rightPassRefine' c Q \<equiv> do {
     (c, _) \<leftarrow> WHILE (\<lambda>(c, Q). Q \<noteq> {}) (\<lambda>(c, Q). do {
       e \<leftarrow> SPEC (\<lambda>e. e \<in> Q);
       let Q = Q - {e};
       let v = snd e;
       if Graph.incoming c v = {} then do {
-        let Q = Q \<union> Graph.outgoing c v;
-        let c = removeEdge c e;
+        let R = Graph.outgoing c v;
+        let Q = Q \<union> R;
+        let c = removeEdges c R;
         RETURN (c, Q)}
       else RETURN (c, Q)
     }) (c, Q);
     RETURN c
   }"
+
+text \<open>This definition is slightly adapted in that it works on the set of edge tails,
+      instead of on the edges themselves.\<close>
+definition rightPassRefine :: "_ graph \<Rightarrow> node set \<Rightarrow> (_ graph) nres" where
+  "rightPassRefine c Q \<equiv> do {
+    (c, _) \<leftarrow> WHILE (\<lambda>(c, Q). Q \<noteq> {}) (\<lambda>(c, Q). do {
+      u \<leftarrow> SPEC (\<lambda>u. u \<in> Q);
+      let Q = Q - {u};
+      if Graph.incoming c u = {} then do {
+        let R = Graph.outgoing c u;
+        let Q = Q \<union> (snd ` R);
+        let c = removeEdges c R;
+        RETURN (c, Q)}
+      else RETURN (c, Q)
+    }) (c, Q);
+    RETURN c
+  }"
+
+(* TODO check which definition is better *)
+
+(*definition non_s_nodes_outside_Q_have_in :: "node \<Rightarrow> (_ graph \<times> node set) \<Rightarrow> bool"
+  where "non_s_nodes_outside_Q_have_in s \<equiv> \<lambda>(c, Q). \<forall>u \<in> Graph.V c - Q - {s}. Graph.incoming c u \<noteq> {}"*)
+
+definition rightPass_invar :: "_graph \<Rightarrow> node \<Rightarrow> (_ graph \<times> node set) \<Rightarrow> bool"
+  where "rightPass_invar c s \<equiv> \<lambda>(c', Q). isSubgraph c' c \<and> (\<forall>u \<in> Graph.V c' - Q - {s}. Graph.incoming c' u \<noteq> {})"
+(* TODO include subgraph *)
+
+thm rightPassAbstract_def
+thm Graph.outgoing'_def
+thm subgraph.order_antisym
+
+find_theorems "(?a \<noteq> 0 \<Longrightarrow> ?a = ?b) \<Longrightarrow> (?b \<noteq> 0 \<Longrightarrow> ?a = ?b) \<Longrightarrow> ?a = ?b"
+
+(* TODO check whether the distance bound is really necessary (it should be) *)
+context Distance_Bounded_Graph
+begin
+
+lemma rightPassRefine_correct:
+  (* TODO make sure the assumptions are correct *)
+  assumes "s \<notin> Q" and NODE_HAS_IN: "\<forall>u \<in> V - Q - {s}. incoming u \<noteq> {}"
+  shows "rightPassRefine c Q \<le> RETURN (rightPassAbstract c s)"
+  unfolding rightPassRefine_def
+proof (intro WHILE_rule[where I="rightPass_invar c s"] refine_vcg, clarsimp_all)
+  show "rightPass_invar c s (c, Q)" unfolding rightPass_invar_def using NODE_HAS_IN by blast
+next
+  fix c' :: "'capacity graph"
+  fix Q u
+  assume "rightPass_invar c s (c', Q)" "u \<in> Q"
+  show "Graph.incoming c' u = {} \<Longrightarrow> rightPass_invar c s (removeEdges c' (Graph.outgoing c' u), Q - {u} \<union> snd ` Graph.outgoing c' u)" sorry
+  show "Graph.incoming c' u \<noteq> {} \<Longrightarrow> rightPass_invar c s (c', Q - {u})" sorry
+next
+  fix c' :: "'capacity  graph"
+  assume "rightPass_invar c s (c', {})"
+  then have "isSubgraph c' c" "\<forall>u \<in> Graph.V c' - {s}. Graph.incoming c' u \<noteq> {}"
+    unfolding rightPass_invar_def by simp_all
+  then interpret c'_sub_c: Subgraph c' c by unfold_locales
+  interpret g': Distance_Bounded_Graph c' b
+    using c'_sub_c.sg_Distance_Bounded Distance_Bounded_Graph_axioms by blast (* TODO necessary* *)
+  show "rightPassAbstract c s = c'" unfolding rightPass_invar_def
+  (*proof (intro ext, clarify)*)
+  proof (intro subgraph.order_antisym, unfold isSubgraph_def, clarsimp_all)
+    fix u v
+    assume "rightPassAbstract c s (u, v) \<noteq> 0"
+    then show "rightPassAbstract c s (u, v) = c' (u, v)" sorry (* TODO this will fail, assumption about maintaining s-connected nodes missing *)
+  next
+    fix u v
+    assume "c' (u, v) \<noteq> 0"
+    then obtain w p where "Graph.isPath c' w p u" "Graph.incoming c' w = {}" using g'.obtain_front_terminal_path by blast
+    then show "c' (u, v) = rightPassAbstract c s (u, v)" sorry
+  qed
+qed
+end
 
 \<comment> \<open>RightPass\<close>
 
